pcuic/theories/PCUICInductiveInversion.v
@@ -15,7 +15,7 @@ From MetaCoq.PCUIC Require Import PCUICAst PCUICAstUtils PCUICTactics PCUICInduc
      PCUICConversion PCUICInversion PCUICContexts PCUICArities
      PCUICSpine PCUICInductives PCUICWellScopedCumulativity PCUICValidity.
 
-From MetaCoq.PCUIC Require Import PCUICParallelReductionConfluence.
+From MetaCoq.PCUIC Require PCUICParallelReductionConfluence.
 (* for nth_error lemma. should move *)
 
 Require Import Equations.Type.Relation_Properties.
@@ -952,9 +952,9 @@ Proof.
   congruence.
 Qed.
 
-Lemma Proj_Construct_ind_eq {cf:checker_flags} Σ (hΣ : ∥ wf Σ.1 ∥) {Γ i i' pars narg c u l T} :
-  Σ ;;; Γ |- tProj (i, pars, narg) (mkApps (tConstruct i' c u) l) : T ->
-  i = i'.
+Lemma Proj_Construct_ind_eq {cf:checker_flags} Σ (hΣ : ∥ wf Σ.1 ∥) {Γ i' p c u l T} :
+  Σ ;;; Γ |- tProj p (mkApps (tConstruct i' c u) l) : T ->
+  p.(proj_ind) = i'.
 Proof.
   destruct hΣ as [wΣ].
   intros h.
@@ -967,9 +967,9 @@ Proof.
   intuition auto.
 Qed.
 
-Lemma invert_Proj_Construct {cf:checker_flags} Σ (hΣ : ∥ wf Σ.1 ∥) {Γ i i' pars narg c u l T} :
-  Σ ;;; Γ |- tProj (i, pars, narg) (mkApps (tConstruct i' c u) l) : T ->
-  i = i' /\ c = 0 /\ pars + narg < #|l|.
+Lemma invert_Proj_Construct {cf:checker_flags} Σ (hΣ : ∥ wf Σ.1 ∥) {Γ p i' c u l T} :
+  Σ ;;; Γ |- tProj p (mkApps (tConstruct i' c u) l) : T ->
+  p.(proj_ind) = i' /\ c = 0 /\ p.(proj_npars) + p.(proj_arg) < #|l|.
 Proof.
   intros h.
   assert (h' := h).
@@ -990,8 +990,8 @@ Proof.
   set (oib := declared_inductive_inv _ _ _ _) in *.
   simpl in *.
   destruct declc.
-  destruct p0 as [[[? ?] ?] ?].
-  destruct p.
+  destruct p1 as [[[? ?] ?] ?].
+  destruct p0.
   destruct (ind_cunivs oib) as [|? []] eqn:hctor in y; try contradiction.
   simpl in H. simpl in H0.
   rewrite e0 in H0.
@@ -1549,7 +1549,7 @@ Proof.
       inductive_mind := inductive_mind ind;
       inductive_ind := Nat.pred #|ind_bodies mdecl| - (k - #|ctx|) |} mdecl i).
       { split; auto. simpl. rewrite -e nth_error_rev; lia_f_equal. }
-      rewrite (declared_inductive_lookup_inductive H0) //.
+      rewrite (declared_inductive_lookup H0) //.
       destruct (on_declared_inductive H0) as [onmind onind] => //. simpl in *.
       rewrite e0 /ind_realargs /PCUICTypingDef.destArity.
       rewrite !onind.(ind_arity_eq).
@@ -1722,70 +1722,6 @@ Proof.
   econstructor 2. eapply r. auto.
 Qed.
 
-Lemma nth_error_decl_body_ass_ctx {Γ Δ i body} : 
-  assumption_context Γ ->
-  option_map decl_body (nth_error (Γ ,,, Δ) i) = Some (Some body) ->
-  i < #|Δ|.
-Proof.
-  intros ass.
-  destruct nth_error eqn:eq.
-  simpl.
-  destruct (i <? #|Δ|) eqn:lt.
-  eapply Nat.ltb_lt in lt => //.
-  eapply Nat.ltb_nlt in lt => //.
-  rewrite nth_error_app_ge in eq. lia.
-  eapply nth_error_assumption_context in eq; eauto. rewrite eq //.
-  by [].
-Qed.
-  
-(*Lemma red1_assumption_context_irrelevant Σ Γ Δ Γ' t t' : 
-  red1 Σ (Γ ,,, Δ) t t' ->
-  assumption_context Γ ->
-  #|Γ| = #|Γ'| ->
-  red1 Σ (Γ' ,,, Δ) t t'. 
-Proof.
-  (* subsummed by red_type_irrelevance *)
-  (*remember (Γ ,,, Δ) as ctx.
-  intros H; revert Γ Δ Heqctx Γ'. 
-  induction H using red1_ind_all; intros; subst; try solve [econstructor; eauto; try solve_all].
-  
-  - pose proof (nth_error_decl_body_ass_ctx H0 H).
-    rewrite nth_error_app_lt // in H |- *.
-    constructor. rewrite nth_error_app_lt //.
-  - econstructor; eauto; eapply (IHred1 Γ0 (Δ ,, vass na N) ltac:(reflexivity)) => //.
-  - econstructor; eauto; eapply (IHred1 Γ0 (Δ ,, vdef na b t) ltac:(reflexivity)) => //.
-  - econstructor; eauto; eapply (IHred1 Γ0 (Δ ,, vass na M1) ltac:(reflexivity)) => //.
-  - eapply fix_red_body. solve_all.
-    specialize (b0 Γ0 (Δ ,,, fix_context mfix0) ltac:(rewrite app_context_assoc; reflexivity) _ H H0).
-    now rewrite app_context_assoc in b0.
-  - eapply cofix_red_body. solve_all.
-    specialize (b0 Γ0 (Δ ,,, fix_context mfix0) ltac:(rewrite app_context_assoc; reflexivity) _ H H0).
-    now rewrite app_context_assoc in b0.*)
-Qed.
-
-Lemma red_assumption_context_app_irrelevant Σ Γ Δ Γ' t t' : 
-  red Σ (Γ ,,, Δ) t t' ->
-  assumption_context Γ ->
-  #|Γ| = #|Γ'| ->
-  red Σ (Γ' ,,, Δ) t t'. 
-Proof.
-  intros r ass eqc.
-  eapply clos_rt_rt1n in r.
-  eapply clos_rt1n_rt.
-  induction r; [constructor|econstructor 2].
-  eapply red1_assumption_context_irrelevant; eauto. apply IHr.
-Qed.
-
-Lemma red_assumption_context_irrelevant Σ Γ Γ' t t' : 
-  red Σ Γ t t' ->
-  assumption_context Γ ->
-  #|Γ| = #|Γ'| ->
-  red Σ Γ' t t'. 
-Proof.
-  intros r ass eqc.
-  now eapply (red_assumption_context_app_irrelevant _ _ [] Γ').
-Qed.
-*)
 Lemma assumption_context_map f Γ :
   assumption_context Γ -> assumption_context (map_context f Γ).
 Proof.
@@ -2451,7 +2387,7 @@ Proof.
     eapply closedn_ctx_upwards; tea. lia. }
   destruct global_variance eqn:gv.
   { move:gv.
-    simpl. rewrite (declared_inductive_lookup_inductive decli).
+    simpl. rewrite (declared_inductive_lookup decli).
     rewrite oib.(ind_arity_eq). 
     rewrite !destArity_it_mkProd_or_LetIn. simpl.
     rewrite app_context_nil_l context_assumptions_app.
@@ -2679,7 +2615,7 @@ Proof.
   { apply spine_codom_wf in spu'; eauto with fvs. }
   destruct global_variance eqn:gv.
   { move:gv.
-    simpl. rewrite (declared_inductive_lookup_inductive declc).
+    simpl. rewrite (declared_inductive_lookup declc).
     rewrite oib.(ind_arity_eq). 
     rewrite !destArity_it_mkProd_or_LetIn. simpl.
     rewrite app_context_nil_l context_assumptions_app.
@@ -3068,9 +3004,9 @@ Lemma projection_cumulative_indices {cf} {Σ} {wfΣ : wf Σ} :
   on_udecl_prop Σ (ind_universes mdecl) ->
   consistent_instance_ext Σ (ind_universes mdecl) u ->
   consistent_instance_ext Σ (ind_universes mdecl) u' ->
-  R_global_instance Σ (eq_universe Σ) (leq_universe Σ) (IndRef p.1.1) (ind_npars mdecl) u u' ->
-  Σ ;;; projection_context p.1.1 mdecl idecl u ⊢
-    subst_instance u pdecl.2 ≤ subst_instance u' pdecl.2.
+  R_global_instance Σ (eq_universe Σ) (leq_universe Σ) (IndRef p.(proj_ind)) (ind_npars mdecl) u u' ->
+  Σ ;;; projection_context p.(proj_ind) mdecl idecl u ⊢
+    subst_instance u pdecl.(proj_type) ≤ subst_instance u' pdecl.(proj_type).
 Proof.
   intros * declp onudecl cu cu' Ru.
   epose proof (declared_projection_constructor declp) as declc.
@@ -3199,16 +3135,16 @@ Proof.
   move: Hty; rewrite subst_context_nil /=.
   rewrite skipn_length. len. simpl. len.
   rewrite /projection_type /=.
-  fold (expand_lets_k (ind_params mdecl) p.2 ty).
+  fold (expand_lets_k (ind_params mdecl) p.(proj_arg) ty).
   rewrite projs_inst_skipn.
   assert (context_assumptions (cstr_args cdecl) - 
-    S (context_assumptions (cstr_args cdecl) - S p.2) = p.2) as -> by lia.
+    S (context_assumptions (cstr_args cdecl) - S p.(proj_arg)) = p.(proj_arg)) as -> by lia.
   clear X.
   rewrite subst_instance_subst.
   rewrite (subst_instance_subst u').
   rewrite !subst_instance_subst [subst_instance _ (projs _ _ _)]subst_instance_projs.
   rewrite - !subst_instance_subst.
-  fold (expand_lets_k (ind_params mdecl) p.2 ty).
+  fold (expand_lets_k (ind_params mdecl) p.(proj_arg) ty).
   rewrite commut_lift_subst_rec => /lens.
   rewrite commut_lift_subst_rec => /lens.
   rewrite distr_subst projs_subst_above. lia.
@@ -3262,7 +3198,7 @@ Lemma ctx_inst_app_weak `{checker_flags} Σ (wfΣ : wf Σ.1) ind mdecl idecl (is
 Proof.
   intros [? ty_args] ? cparams cum.
   pose proof (wt_ind_app_variance (x; ty_args)) as [mdecl' [idecl' gv]].
-  rewrite (declared_inductive_lookup_inductive isdecl) in idecl'. noconf idecl'.
+  rewrite (declared_inductive_lookup isdecl) in idecl'. noconf idecl'.
   eapply invert_type_mkApps_ind in ty_args as [ty_args ?] ; eauto.
   erewrite ind_arity_eq in ty_args.
   2: eapply PCUICInductives.oib ; eauto.
