pcuic/theories/PCUICValidity.v
@@ -411,7 +411,6 @@ Section Validity.
     - (* Proj *)
       pose proof isdecl as isdecl'.
       eapply declared_projection_type in isdecl'; eauto.
-      subst ty.
       destruct isdecl' as [s Hs].
       unshelve eapply isType_mkApps_Ind_inv in X2 as [parsubst [argsubst [sppar sparg 
         lenpars lenargs cu]]]; eauto.
