pcuic/theories/utils/PCUICAstUtils.v
@@ -35,8 +35,8 @@ Fixpoint string_of_term (t : term) :=
   | tCase ci p t brs =>
     "Case(" ^ string_of_case_info ci ^ "," ^ string_of_term t ^ ","
             ^ string_of_predicate string_of_term p ^ "," ^ string_of_list (string_of_branch string_of_term) brs ^ ")"
-  | tProj (ind, i, k) c =>
-    "Proj(" ^ string_of_inductive ind ^ "," ^ string_of_nat i ^ "," ^ string_of_nat k ^ ","
+  | tProj p c =>
+    "Proj(" ^ string_of_inductive p.(proj_ind) ^ "," ^ string_of_nat p.(proj_npars) ^ "," ^ string_of_nat p.(proj_arg) ^ ","
             ^ string_of_term c ^ ")"
   | tFix l n => "Fix(" ^ (string_of_list (string_of_def string_of_term) l) ^ "," ^ string_of_nat n ^ ")"
   | tCoFix l n => "CoFix(" ^ (string_of_list (string_of_def string_of_term) l) ^ "," ^ string_of_nat n ^ ")"
